---
id: "sister-tear-ship"
created: "Sun Apr 27 19:02:20 2025"
attribution: TBA
---

```{r include=FALSE, eval=!"devoirs" %in% (.packages())}
# For stand-alone compilation testing
library(devoirs)
library(mosaicCalc)
```

::: {#exr-sister-tear-ship}


Part 1  
: Simplify $\int_{t}^{-t}1\ dt$

<!-- Opening answer: sts-2KX -->
::: {.callout-tip collapse=true `r answer_style()`}
## Answer
The anti-derivative $G(t) = \int 1 dt = t + C$. Evaluating $G()$ at the limits of integration gives $$G(t) - G(-t) = t + C - \left[-t + C\right] - 2\,t\. $$

We have include the "constant of integration" $C$ here for completeness, but when the calculation is going to involve $G(upper) - G(lower)$, the constants of integration will *always* cancal out.

[..id..]{data-tooltip="Ans id: sts-2KX"}
:::
<!-- closing answer sts-2KX -->


Part 2  
: $\int_a^b 1 dx$

<!-- Opening answer: sts-3sW -->
::: {.callout-tip collapse=true `r answer_style()`}
## Answer
The anti-derivative $G(t) = \int 1 dx = x + C$. Evaluating $G()$ at the limits of integration gives $G(b) - G(a) = b + C - [a + C] = b - a\ .$$

Again, we've put in the constant of integration C explicitly, but we'll stop now since all the calculations below involve $G(upper) - G(lower)$ where the constants of integration will cancel out.
[..id..]{data-tooltip="Ans id: sts-3sW"}
:::
<!-- closing answer sts-3sW -->


Part 3  
: $\int_0^x 3 t^2\ dt$

<!-- Opening answer: sts-7Ks -->
::: {.callout-tip collapse=true `r answer_style()`}
## Answer
Happily, we recognize the integrand, $3 t^2$, as the derivative of the function $t^3$. So $G(t) = t^3$. (We're leaving out the constant of integration $C$ for the reason described in the previous answer blocks.)

Evaluating $G()$ at the upper and lower limits of integration gives $$G(x) - G(0)\ .$$

[..id..]{data-tooltip="Ans id: sts-7Ks"}
:::
<!-- closing answer sts-7Ks -->


Part 4  
: $\int_a^b f(x)\ dx + \int_b^a f(y)\ dy$

<!-- Opening answer: sts-9go -->
::: {.callout-tip collapse=true `r answer_style()`}
## Answer
Some things to notice:

1. The name of the with-respect-to variable doesn't matter so the second integral is the same as the first integral but with the limits of integration flipped around.
2. Even though we don't know $f(x)$, we can still make progress. Let's call $\int f(x) dx$ by the name $F(x)$. We don't know $F()$ but we can still formally evaluate it at the limits of integration:

$$F(b) - F(a) - \left[F(b) - F(a)\right] = 0\ .$$


[..id..]{data-tooltip="Ans id: sts-9go"}
:::
<!-- closing answer sts-9go -->

Part 5  
: $\int_1^x \frac{1}{t}\ dt$

<!-- Opening answer: sts-7Wa -->
::: {.callout-tip collapse=true `r answer_style()`}
## Answer
With luck, you'll recognize the function $1/t$ as the derivative of $\ln(t)$. Consequently, we know that $G(t) \equiv \ln(t)$. (Again, leaving out the constant of integration since we have both lower and upper limits of integration.) Overall, the result: $$G(x) - G(1) = \ln(x) - \ln(1) = \ln(x)\ .$$

[..id..]{data-tooltip="Ans id: sts-7Wa"}
:::
<!-- closing answer sts-7Wa -->


Part 6  
: $\int_0^{t^2} \omega \cos(\omega t)\ dt$ -> $\sin(\omega t^2)$

<!-- Opening answer: sts-6lO -->
::: {.callout-tip collapse=true `r answer_style()`}
## Answer
How nice! $\omega \cos(\omega t)$ is the derivative of the basic modeling function $\sin(\omega t)$. Correspondingly, $G(t) = \sin(\omega t)$. Evaluating at the limits of integration gives $$\sin(\omega t^2) - \sin(\omega 0) = \sin(\omega t^2)\ .$$

It may seem odd to have a limit of integration be a compound expresssion like $t^2$, but any expression can serve as a limit of integration.

[..id..]{data-tooltip="Ans id: sts-6lO"}
:::
<!-- closing answer sts-6lO -->


Part 7  
: $\partial_x \int x \text{dnorm}(x)\ dx$ 

<!-- Opening answer: sts-3Ea -->
::: {.callout-tip collapse=true `r answer_style()`}
## Answer
There seems to be a pattern among these exercises: the integrands have been selected to give simple results since they are the derivatives of pattern-book functions.

Here, the integrand is the derivative of $\text{dnorm}(x)$ so the anti-derivative is $G(x) = \text{dnorm}(x)$. Taking the derivative $\partial_x G(x)$ gives $x \text{dnorm}(x)$. 

Even simpler, we can recognize the $\partial_x$ as undoing the $\int f(x) dx$, so the result is just the integrand.


[..id..]{data-tooltip="Ans id: sts-3Ea"}
:::
<!-- closing answer sts-3Ea -->

Part 8  
: $\partial_t \int_0^x pnorm(x)\ dx$

<!-- Opening answer: sts-5MN -->
::: {.callout-tip collapse=true `r answer_style()`}
## Answer
A trick here! We don't actually know the anti-derivative of $\text{pnorm}(x)$, but let's just call it $G()$ so the integral is $G(x) - G(0)$. Neither of these is a function of $t$, so the overall expression is simply zero.


[..id..]{data-tooltip="Ans id: sts-5MN"}
:::
<!-- closing answer sts-5MN -->

Part 9  
: $\int e^{a + bt}\ dt$

<!-- Opening answer: sts-9vA -->
::: {.callout-tip collapse=true `r answer_style()`}
## Answer
Let's re-write this with a simplified integrand:

$$\int e^{a + bt}\ dt = \int e^a e^{bt}\ dt = e^a \int e^{bt}\ dt$$
Now $e^{bt}$ isn't the derivative of a pattern-book function, but it's close! $b e^{bt}$ is the derivative of $e^{bt}$. The trick is to recognize that $e^{bt} = \frac{b}{b} e^{bt}$ so

$$e^a \int e^{bt}\ dt = e^a \int \frac{b}{b} e^{bt}\ dt = \frac{e^a}{b} \int b e^{bt}\ dt = \frac{e^a}{b} e^{bt} = \frac{1}{b}e^{a + bt}$$


[..id..]{data-tooltip="Ans id: sts-9vA"}
:::
<!-- closing answer sts-9vA -->

:::
 <!--Part 1  : end of exr-sister-tear-ship -->
